theories/STS.v
@@ -19,13 +19,7 @@ Record semantics : Type := Semantics_gen {
   state_sort: state -> sort;
   (* wf_vis: forall st0 (VIS: state_sort st0 = vis), exists ! ev st1, step st0 (Some ev) st1; *)
   (* wf_vis: forall st0 (VIS: state_sort st0 = vis), exists ev st1, step st0 (Some ev) st1; *)
-  (* wf_vis: forall *)
-  (*     st0 ev0 ev1 st1 st2 *)
-  (*     (VIS: state_sort st0 = vis) *)
-  (*     (STEP: step st0 ev0 st1) *)
-  (*     (STEP: step st0 ev1 st2) *)
-  (*   , *)
-  (*     ev0 = ev1 /\ st1 = st2; *)
+  (** wf_vis might be completely removed with a new transformation pass *)
   wf_vis: forall
       st0 ev0 ev1 st1 st2
       (VIS: state_sort st0 = vis)
