theories/Universe.v
@@ -186,6 +186,4 @@ Definition unint (v: val): option Z :=
 (*** NOTE: Probably we can support comparison between nullptr and 0 ***)
 (*** NOTE: Unlike CompCert, we don't support comparison with weak_valid_ptr (for simplicity) ***)
 
-(* Parameter syscall_sem: gname -> list val -> (event * val). *)
-(* Parameter syscall_sem: gname -> list val -> event. *)
 Parameter syscall_sem: event -> Prop.
